feat: (almost) add substitutions lemmas for CPSFix

PyroLeanExamples/Basic.lean
@@ -191,7 +191,8 @@ modular (name := `STLCFix)
       | _, _, .fix e => .fix (Expr.subst σ.lift.lift e)
 
   inductive Equiv extends STLC.Equiv where
-    | fix : Equiv (.app (.ret (.fix e)) (.ret v)) (e.subst (Sub.id |>.snoc (.fix e) |>.snoc v))
+    | fix : Equiv e e' → Equiv (.fix e) (.fix e')
+    | fix_red : Equiv (.app (.ret (.fix e)) (.ret v)) (e.subst (Sub.id |>.snoc (.fix e) |>.snoc v))
 end STLCFix
 
 modular (name := `STLCBool)
@@ -363,6 +364,274 @@ modular (name := `CPS)
   mod def Equiv.equiv extends Base.Equiv.equiv
   mod def Equiv.setoid extends Base.Equiv.setoid
 
+
+def Ren.comp (r₁ : Ren Γ Δ) (r₂ : Ren Δ Φ) : Ren Γ Φ where
+  val := r₁.val ∘ r₂.val
+  property n := r₂.property n |>.trans (r₁.property (r₂.val n))
+
+theorem Expr.ren_of_ren_ren  {r₁ : Ren Γ Δ} {r₂ : Ren Δ Φ} (v : Expr Φ t A) : (v.ren r₂).ren r₁ = v.ren (r₁.comp r₂) := by
+  induction v generalizing r₁ Γ Δ <;> simp [ren, Ren.comp, *]
+  case lam =>
+    congr 2
+    funext ⟨x,_⟩
+    cases x <;> rfl
+  case and_elim =>
+    congr 2
+    funext ⟨x,_⟩
+    cases x
+    case zero => rfl
+    case succ x _ => cases x <;> rfl
+
+theorem Expr.ren_lift_wk {r : Ren Γ Δ} : (r.lift.comp Ren.wk) = ((Ren.wk (A := B)).comp r) := by
+  simp [Ren.comp, Ren.lift, Ren.wk]
+  rfl
+
+theorem Expr.lift_ren_lift {r : Ren Γ Δ} (v : Expr Δ t A): Expr.ren r.lift v.lift = (Expr.ren r v).lift (B := B) := by
+  rw [Expr.lift, Expr.lift, Expr.ren_of_ren_ren, Expr.ren_of_ren_ren]
+  rfl
+
+def Sub.ren_comp (ρ : Ren Γ Δ) (σ : Sub Δ Φ) : Sub Γ Φ := fun n =>
+  (σ n).ren ρ
+
+def Sub.comp_ren (σ : Sub Γ Δ) (ρ : Ren Δ Φ) : Sub Γ Φ := fun n =>
+  (ρ.2 n) ▸ σ (ρ.val n)
+
+@[simp]
+theorem Sub.snoc_comp_ren_wk (σ : Sub Γ Δ) : (σ.snoc t).comp_ren .wk = σ := rfl
+
+def Sub.comp (σ₁ : Sub Γ Δ) (σ₂ : Sub Δ Φ) : Sub Γ Φ :=
+  fun n => (σ₂ n).subst σ₁
+
+@[simp]
+theorem Sub.wk_snoc_zero (σ : Sub Γ Δ) : (σ.wk (A := A)).snoc Expr.zero = σ.lift := rfl
+
+@[simp]
+theorem Expr.subst_lift_zero (σ : Sub Γ Δ) : σ.lift (A := A) ⟨0,h⟩ = Expr.zero := rfl
+
+@[simp]
+theorem Expr.subst_snoc_zero (σ : Sub Γ Δ) : σ.snoc e ⟨0,h⟩ = e := rfl
+
+@[simp]
+theorem Expr.subst_snoc_succ (σ : Sub Γ Δ) : σ.snoc e ⟨n+1,h⟩ = σ ⟨n,Nat.lt_of_succ_lt_succ h⟩ := rfl
+
+@[simp]
+theorem Expr.subst_lift_succ (σ : Sub Γ Δ) : σ.lift (A := A) ⟨n+1,h⟩ = (σ ⟨n,Nat.lt_of_succ_lt_succ h⟩).lift := rfl
+
+theorem Sub.ren_comp_lift {r : Ren Γ Δ} {σ : Sub Δ Φ} : (σ.ren_comp r).lift (A := A) = σ.lift.ren_comp r.lift  := by
+  funext ⟨x,_⟩
+  simp
+  cases x
+  · rfl
+  · simp [ren_comp, Expr.lift, Expr.ren_of_ren_ren]
+    rfl
+
+theorem Sub.wk_of_lift_comp_ren_wk {σ : Sub Γ Δ} : (σ.lift.comp_ren Ren.wk) = σ.wk (A := A) := by
+  funext ⟨x,_⟩
+  rw [comp_ren, Sub.wk, Expr.lift, Ren.wk]
+  simp only
+  unfold Fin.succ
+  rw [Expr.subst_lift_succ, Expr.lift]
+
+theorem Sub.head (σ : Sub Γ Δ) : Expr.subst (σ.snoc t) Expr.zero = t := rfl
+theorem Sub.tail (σ : Sub Γ Δ) : (σ.snoc t).comp Sub.id.wk = σ := rfl
+
+theorem Sub.eta (σ : Sub Γ (A::Δ)) : (σ.comp Sub.id.wk).snoc (σ 0) = σ := by
+  funext ⟨n,_⟩
+  cases n <;> rfl
+
+theorem Sub.Zshift' : Sub.id.wk.snoc Expr.zero = @Sub.id (A::Γ) := by
+  funext ⟨n,_⟩
+  cases n <;> rfl
+
+theorem Sub.Zshift : Sub.id.lift = @Sub.id (A::Γ) := Zshift'
+
+theorem Sub.idR (σ : Sub Γ Δ) : (σ.comp Sub.id) = σ := rfl
+
+@[simp]
+theorem Expr.subst_id : Expr.subst Sub.id t = t := by
+  induction t <;> simp [Sub.Zshift, subst, *]
+  case var h => cases h; rfl
+
+@[simp]
+theorem Sub.idL (σ : Sub Γ Δ) : Sub.comp Sub.id σ = σ := by
+  funext n
+  apply Expr.subst_id
+
+theorem Expr.subst_comp_ren_lift (σ : Sub Δ Γ ) (ρ : Ren Φ Δ) : (σ.ren_comp ρ).lift (A := A) = (σ.lift.ren_comp ρ.lift ) := by
+  funext ⟨n,_⟩
+  cases n
+  · rfl
+  · simp [Sub.ren_comp, Expr.lift, ren_of_ren_ren]
+    rfl
+
+theorem Expr.subst_ren (t : Expr Φ t A) (ρ : Ren Γ Δ) (σ : Sub Δ Φ) : (t.subst σ).ren ρ = t.subst (σ.ren_comp ρ) := by
+  induction t generalizing ρ Γ Δ <;> simp [Sub.ren_comp, ren, subst, *]
+  case var h => cases h; rfl
+  case lam ih =>
+    rw [Expr.subst_comp_ren_lift]
+  case and_elim ih₁ ih₂ =>
+    rw [Expr.subst_comp_ren_lift, Expr.subst_comp_ren_lift]
+
+@[simp]
+theorem Ren.lift_succ (ρ : Ren Γ Δ) : (ρ.lift (A := A)).val ⟨n+1,h⟩ = (ρ.val ⟨n, Nat.lt_of_succ_lt_succ h⟩).succ := rfl
+
+@[simp]
+theorem Sub.lift_succ (σ : Sub Γ Δ) : (σ.lift (A := A)) n.succ = (σ n).lift := rfl
+
+--  ext-ren-sub-∘≣, just cases n <;> rfl in agda *somehow*
+theorem Expr.ren_comp_subst_lift (ρ : Ren Δ Γ) (σ : Sub Φ Δ) : (σ.comp_ren ρ).lift (A := A) = (σ.lift.comp_ren ρ.lift) := by
+  funext ⟨n,_⟩
+  cases n
+  case zero => rfl
+  case succ n h =>
+    simp [Sub.comp_ren, Expr.lift]
+    grind only [usr Subtype.property]
+
+theorem Expr.ren_subst (t : Expr Φ t A) (σ : Sub Γ Δ) (ρ : Ren  Δ Φ) : (t.ren ρ).subst σ = t.subst (Sub.comp_ren σ ρ) := by
+  induction t generalizing σ Γ Δ <;> simp [Sub.comp_ren, ren, subst, *]
+  case var h => cases h; rfl
+  case lam ih =>
+    have := ih σ.lift ρ.lift
+    rw [← this, ren_comp_subst_lift]
+    assumption
+  case and_elim ih₁ ih₂ =>
+    rw [ren_comp_subst_lift, ren_comp_subst_lift]
+
+theorem Expr.lift_subst_lift (t : Expr Δ t B) (σ : Sub Γ Δ) :
+(t.lift (A := B)).subst σ.lift = (t.subst σ).lift (B := A) := by
+  induction t <;> simp [Expr.lift, Expr.ren, Expr.subst] at *
+  case var h => cases h; rfl
+  case lam ih =>
+    rw [Expr.subst_ren, ← Expr.subst_comp_ren_lift, Expr.ren_subst, ← Expr.ren_comp_subst_lift]
+    rfl
+  case and_elim ih₁ ih₂ =>
+    constructor
+    · rw [Expr.subst_ren, Expr.ren_subst]
+      rfl
+    · rw [Expr.subst_ren, ← Expr.subst_comp_ren_lift, Expr.ren_subst, ← Expr.ren_comp_subst_lift, ← Expr.ren_comp_subst_lift , ← Expr.subst_comp_ren_lift]
+      congr 1
+  case app ih₁ ih₂ | and_intro ih₁ ih₂ => exact ⟨ih₁ _, ih₂ _⟩
+
+@[simp]
+theorem Sub.comp_lift {σ : Sub Γ Δ} {τ : Sub Δ Φ} : Sub.comp σ.lift τ.lift = (Sub.comp σ τ).lift (A := A) := by
+  funext ⟨x,_⟩
+  cases x --generalizing  Γ Δ Φ
+  case zero => rfl
+  case succ n h =>
+    simp [Sub.comp, Expr.lift, Expr.ren_subst , Expr.subst_ren]
+    rfl
+
+theorem Expr.subst_subst  {σ₁ : Sub Γ Δ} {σ₂ : Sub Δ Φ} (v : Expr Φ t A) : (v.subst σ₂).subst σ₁ = v.subst (σ₁.comp σ₂) := by
+  induction v generalizing σ₁ Γ Δ <;> simp only [subst, Fin.getElem_fin, Sub.comp, *]
+  case var h =>
+    cases h
+    rfl
+  case lam A Φ t ih =>
+    rw [Sub.comp_lift]
+  case and_elim ih =>
+    rw [Sub.comp_lift, Sub.comp_lift]
+
+theorem Expr.cast_val {h : Γ[n] = A}(e : A = B) : e ▸ Expr.var n h = Expr.var n h' := by cases e; rfl
+
+theorem Equiv.ren {r : Ren Γ Δ} (e₁ e₂ : Expr Δ t A) : Equiv e₁ e₂ → Equiv (e₁.ren r) (e₂.ren r) := by
+  intro h
+  induction h generalizing Γ
+  case refl => exact .refl
+  case symm ih => exact .symm ih
+  case trans ih₁ ih₂ => exact .trans ih₁ ih₂
+  case lam ih => exact Equiv.lam ih
+  case app ih₁ ih₂ => exact Equiv.app ih₁ ih₂
+  case and_intro ih₁ ih₂ => exact Equiv.and_intro ih₁ ih₂
+  case and_elim ih₁ ih₂ => exact Equiv.and_elim ih₁ ih₂
+  case eta v =>
+    simp [Expr.ren, Expr.zero, Expr.lift_ren_lift]
+    exact Equiv.eta (v := (Expr.ren r v))
+  case eta_and Δ t fst snd e =>
+    simp [Expr.ren]
+    apply Equiv.trans
+    · apply Equiv.eta_and
+    · have : (e.ren r.lift.lift).subst ((Sub.id.snoc (Expr.ren r snd)).snoc (Expr.ren r fst)) = (e.subst ((Sub.id.snoc snd).snoc fst)).ren r := by
+        simp [Expr.subst_ren, Expr.ren_subst]
+        congr 1
+        funext ⟨x,_⟩
+        cases x
+        case zero => rfl
+        case succ x h =>
+          cases x
+          · rfl
+          · cbv
+            apply Expr.cast_val
+      rw [this]
+      apply Equiv.refl
+  case beta =>
+    simp [Expr.ren]
+    apply Equiv.trans
+    · apply Equiv.beta
+    · rename_i e v
+      have : (e.ren r.lift).subst (Sub.id.snoc (Expr.ren r v)) = (e.subst (Sub.id.snoc v)).ren r := by
+        simp [Expr.subst_ren, Expr.ren_subst]
+        congr 1
+        funext ⟨x,_⟩
+        cases x
+        case zero => rfl
+        case succ x h =>
+          cbv
+          apply Expr.cast_val
+      rw [this]
+      apply Equiv.refl
+
+theorem Equiv.subst {σ : Sub Γ Δ} (e₁ e₂ : Expr Δ t A)  : Equiv e₁ e₂ → Equiv (e₁.subst σ) (e₂.subst σ) := by
+  intro h
+  induction h generalizing Γ
+  case refl => exact .refl
+  case symm ih => exact .symm ih
+  case trans ih₁ ih₂ => exact .trans ih₁ ih₂
+  case lam ih => exact Equiv.lam ih
+  case app ih₁ ih₂ => exact Equiv.app ih₁ ih₂
+  case and_intro ih₁ ih₂ => exact Equiv.and_intro ih₁ ih₂
+  case and_elim ih₁ ih₂ => exact Equiv.and_elim ih₁ ih₂
+  case eta v =>
+    simp [Expr.subst, Expr.zero, Expr.lift_subst_lift]
+    exact Equiv.eta (v := (Expr.subst σ v))
+  case eta_and =>
+    simp [Expr.subst]
+    apply Equiv.trans
+    · apply Equiv.eta_and
+    · rename_i fst snd e
+      have : (Expr.subst ((Sub.id.snoc (Expr.subst σ snd)).snoc (Expr.subst σ fst)) (Expr.subst σ.lift.lift e)) = (Expr.subst σ (Expr.subst ((Sub.id.snoc snd).snoc fst) e)) := by
+        simp [Expr.subst_subst]
+        congr 1
+        funext ⟨n,_⟩
+        cases n
+        case zero => rfl
+        case succ n _ =>
+          simp [Sub.comp, Sub.lift]
+          cases n
+          · rfl
+          · simp [Sub.id, Expr.subst, Expr.lift, Expr.ren_subst]
+      rw [this]
+      apply Equiv.refl
+  case beta =>
+    simp [Expr.subst]
+    apply Equiv.trans
+    · apply Equiv.beta
+    · rename_i e v
+      have : (Expr.subst (Sub.id.snoc (Expr.subst σ v)) (Expr.subst σ.lift e)) = (Expr.subst σ (Expr.subst (Sub.id.snoc v) e)) := by
+        simp [Expr.subst_subst]
+        congr 1
+        funext ⟨n,_⟩
+        cases n
+        · rfl
+        · simp [Sub.comp, Sub.lift, Sub.id, Expr.subst, Expr.lift, Expr.ren_subst]
+      rw [this]
+      apply Equiv.refl
+
+theorem Equiv.cast  (h₁ : Expr Γ t A = Expr Γ t B) (h₂ : A = B) (e₁ e₂ : Expr Γ t A) : Equiv e₁ e₂ →
+  Equiv (cast h₁ e₁) (cast h₁ e₂) := by
+  cases h₂
+  cases h₁
+  exact id
+
 end CPS
 
 -- #exit
@@ -442,8 +711,131 @@ modular (name := `CPSFix)
   mod def Equiv.equiv extends CPS.Equiv.equiv
   mod def Equiv.setoid extends CPS.Equiv.setoid
 
-end CPSFix
+  mod def Ren.comp._proof_1 extends CPS.Ren.comp._proof_1
+  mod def Ren.comp extends CPS.Ren.comp
 
+  mod def Expr.ren_of_ren_ren extends CPS.Expr.ren_of_ren_ren where finally
+    intro _ _ _ ih _ _ _ _
+    simp [Expr.ren, Ren.comp, *]
+    congr 2
+    funext ⟨x,_⟩
+    cases x
+    case zero => rfl
+    case succ x _ => cases x <;> rfl
+
+  mod def Expr.ren_lift_wk extends CPS.Expr.ren_lift_wk
+
+  mod def Expr.lift_ren_lift extends CPS.Expr.lift_ren_lift
+
+  mod def Sub.ren_comp extends CPS.Sub.ren_comp
+
+  mod def Sub.comp_ren._proof_1 extends CPS.Sub.comp_ren._proof_1
+  mod def Sub.comp_ren extends CPS.Sub.comp_ren
+-- #exit
+  @[simp]
+  mod def Sub.snoc_comp_ren_wk extends CPS.Sub.snoc_comp_ren_wk
+
+  mod def Sub.comp extends CPS.Sub.comp
+
+  @[simp]
+  mod def Sub.wk_snoc_zero extends CPS.Sub.wk_snoc_zero
+
+  @[simp]
+  mod def Expr.subst_lift_zero extends CPS.Expr.subst_lift_zero
+
+  @[simp]
+  mod def Expr.subst_snoc_zero extends CPS.Expr.subst_snoc_zero
+
+  @[simp]
+  mod def Expr.subst_snoc_succ extends CPS.Expr.subst_snoc_succ
+
+  @[simp]
+  mod def Expr.subst_lift_succ extends CPS.Expr.subst_lift_succ
+
+  mod def Sub.ren_comp_lift extends CPS.Sub.ren_comp_lift
+
+  mod def Sub.wk_of_lift_comp_ren_wk extends CPS.Sub.wk_of_lift_comp_ren_wk
+
+  mod def Sub.head extends CPS.Sub.head
+  mod def Sub.tail extends CPS.Sub.tail
+  mod def Sub.eta  extends CPS.Sub.eta
+
+  mod def Sub.Zshift' extends CPS.Sub.Zshift'
+
+  mod def Sub.Zshift extends CPS.Sub.Zshift
+
+  mod def Sub.idR extends CPS.Sub.idR
+
+  @[simp]
+  mod def Expr.subst_id extends CPS.Expr.subst_id where
+    finally
+      intros
+      simp [Expr.subst,Sub.Zshift, *]
+
+  @[simp]
+  mod def Sub.idL extends CPS.Sub.idL
+
+  mod def Expr.subst_comp_ren_lift extends CPS.Expr.subst_comp_ren_lift
+
+  mod def Expr.subst_ren extends CPS.Expr.subst_ren where
+    finally
+      intro _ _ _ ih _ _ _ _
+      simp [Expr.subst, Expr.ren, Expr.subst_comp_ren_lift, *]
+
+  @[simp]
+  mod def Ren.lift_succ extends CPS.Ren.lift_succ
+
+  @[simp]
+  mod def Sub.lift_succ extends CPS.Sub.lift_succ
+
+  -- TODO fix this issue...
+  mod def Expr.ren.hcongr_6' extends CPS.Expr.ren.hcongr_6
+  mod def Expr.ren_comp_subst_lift._proof_1_4 extends CPS.Expr.ren_comp_subst_lift._proof_1_4
+  mod def Expr.ren_comp_subst_lift._proof_1_5 extends CPS.Expr.ren_comp_subst_lift._proof_1_5
+  mod def Expr.ren_comp_subst_lift._proof_1_6 extends CPS.Expr.ren_comp_subst_lift._proof_1_6
+  mod def Expr.ren_comp_subst_lift._proof_1_10 extends CPS.Expr.ren_comp_subst_lift._proof_1_10
+  mod def Expr.ren_comp_subst_lift._proof_1_11 extends CPS.Expr.ren_comp_subst_lift._proof_1_11
+  mod def Expr.ren_comp_subst_lift._proof_1_12 extends CPS.Expr.ren_comp_subst_lift._proof_1_12
+  mod def Expr.ren_comp_subst_lift._proof_1_13 extends CPS.Expr.ren_comp_subst_lift._proof_1_13
+  mod def Expr.ren_comp_subst_lift extends CPS.Expr.ren_comp_subst_lift
+
+  mod def Expr.ren_subst extends CPS.Expr.ren_subst where finally
+    intros
+    simp [Expr.ren, Expr.subst, Expr.ren_comp_subst_lift, *]
+
+  mod def Expr.lift_subst_lift extends CPS.Expr.lift_subst_lift where finally
+    intros
+    simp [Expr.lift, Expr.ren, Expr.subst]
+    rw [Expr.subst_ren, ← Expr.subst_comp_ren_lift, Expr.ren_subst, ← Expr.ren_comp_subst_lift, ← Expr.ren_comp_subst_lift , ← Expr.subst_comp_ren_lift]
+    rfl
+
+  @[simp]
+  mod def Sub.comp_lift extends CPS.Sub.comp_lift
+
+-- #exit
+modular (name := `CPSFix') (imports := #[`CPSFix])
+
+  mod def Expr.subst_subst extends CPS.Expr.subst_subst where finally
+    intros
+    simp only [Sub.comp_lift, Expr.subst, *]
+
+
+  mod def Expr.cast_val._proof_1 extends CPS.Expr.cast_val._proof_1
+  mod def Expr.cast_val extends CPS.Expr.cast_val
+
+  -- mod def Equiv.ren extends CPS.Equiv.ren where finally
+    -- intros
+    -- simp only [subst, Fin.getElem_fin, Sub.comp, *]
+    -- rw [Sub.comp_lift, Sub.comp_lift]
+
+  -- mod def Equiv.subst extends CPS.Equiv.subst where finally
+    -- intros
+    -- sorry
+
+  mod def Equiv.cast extends CPS.Equiv.cast
+
+end CPSFix
+#exit
 def STLC.Tag.toCPS : Tag → CPS.Tag
   | dummy => .dummy
   | val => .val
@@ -453,6 +845,10 @@ def STLC.Ty.toCPS : STLC.Ty → CPS.Ty
   | .arr A B => (A.toCPS.times B.toCPS.not).not
 
 def STLC.Ctx.toCPS (Γ : STLC.Ctx) : CPS.Ctx := Γ.map STLC.Ty.toCPS
+
+@[simp]
+theorem STLC.Ctx.toCPS_length (Γ : STLC.Ctx) : Γ.toCPS.length = Γ.length := by
+  simp [toCPS]
 
 abbrev STLC.ToCtx (Γ : STLC.Ctx) : (t : STLC.Tag) → (A: t.Data) → CPS.Ctx
   | .exp, A => A.toCPS.not::Γ.toCPS
@@ -475,291 +871,31 @@ def STLC.Expr.toCPS : Expr Γ t A → STLC.ToExprType Γ t A
     rw [CPS.Ty.not_not] at e e'
     refine CPS.Expr.app (e.subst CPS.Sub.id.wk) (.and_intro (e'.subst CPS.Sub.id.wk) CPS.Expr.zero)
 
-def CPS.Ren.comp (r₁ : Ren Γ Δ) (r₂ : Ren Δ Φ) : Ren Γ Φ where
-  val := r₁.val ∘ r₂.val
-  property n := r₂.property n |>.trans (r₁.property (r₂.val n))
-
-theorem CPS.Expr.ren_of_ren_ren  {r₁ : Ren Γ Δ} {r₂ : Ren Δ Φ} (v : Expr Φ t A) : (v.ren r₂).ren r₁ = v.ren (r₁.comp r₂) := by
-  induction v generalizing r₁ Γ Δ <;> simp [ren, Ren.comp, *]
-  case lam =>
-    congr 2
-    funext ⟨x,_⟩
-    cases x <;> rfl
-  case and_elim =>
-    congr 2
-    funext ⟨x,_⟩
-    cases x
-    case zero => rfl
-    case succ x _ => cases x <;> rfl
-
-theorem CPS.Expr.ren_lift_wk {r : Ren Γ Δ} : (r.lift.comp Ren.wk) = ((Ren.wk (A := B)).comp r) := by
-  simp [Ren.comp, Ren.lift, Ren.wk]
-  rfl
-
-theorem CPS.Expr.lift_ren_lift {r : Ren Γ Δ} (v : Expr Δ t A): Expr.ren r.lift v.lift = (Expr.ren r v).lift (B := B) := by
-  rw [Expr.lift, Expr.lift, CPS.Expr.ren_of_ren_ren, CPS.Expr.ren_of_ren_ren]
-  rfl
-
-def CPS.Sub.ren_comp (ρ : Ren Γ Δ) (σ : Sub Δ Φ) : Sub Γ Φ := fun n =>
-  (σ n).ren ρ
-
-def CPS.Sub.comp_ren (σ : Sub Γ Δ) (ρ : Ren Δ Φ) : Sub Γ Φ := fun n =>
-  (ρ.2 n) ▸ σ (ρ.val n)
-
 @[simp]
-theorem CPS.Sub.snoc_comp_ren_wk (σ : Sub Γ Δ) : (σ.snoc t).comp_ren .wk = σ := rfl
+theorem STLC.Ctx.getElem_toCPS (Γ : STLC.Ctx) (n : Nat) (h : n < Γ.length) :
+  Γ[n].toCPS = Γ.toCPS[n]'(STLC.Ctx.toCPS_length _ ▸ h) := by
+    induction Γ generalizing n
+    case nil => contradiction
+    case cons head tail ih  =>
+      cases n
+      · simp [toCPS, *] at *
+      · simp [toCPS] at *
 
--- abbrev CPS.Ren.toSub (r : Ren Γ Δ) : Sub Γ Δ := fun n => .var (r.val n) (r.2 n).symm
+def STLC.Ren.toCPS (ρ : Ren Γ Δ) : CPS.Ren Γ.toCPS Δ.toCPS where
+  val n := (ρ.val (n.cast (Ctx.toCPS_length _))).cast (Ctx.toCPS_length _).symm
+  property n := by
+    simp at *
+    rw [← STLC.Ctx.getElem_toCPS, ← STLC.Ctx.getElem_toCPS]
+    congr 1
+    exact ρ.property (n.cast (Ctx.toCPS_length _))
 
--- @[simp]
--- theorem CPS.Ren.toSub_lift (r : Ren Γ Δ) : r.lift.toSub = r.toSub.lift (A := A)  := by
-  -- funext ⟨x,_⟩
-  -- cases x <;> rfl
+def STLC.Sub.toCPS (σ : Sub Γ Δ) : CPS.Sub Γ.toCPS Δ.toCPS := fun n => by
+  have := (σ (Fin.cast (Ctx.toCPS_length _) n)).toCPS
+  simp [ToExprType, ToCtx] at this
+  exact this
 
--- instance : Coe (CPS.Ren Γ Δ) (CPS.Sub Γ Δ) where
-  -- coe := CPS.Ren.toSub
 
--- @[simp]
--- theorem CPS.Expr.ren_of_subst_ren {r : Ren Γ Δ} (e : Expr Δ t A) : e.subst r = e.ren r := by
-  -- induction e generalizing Γ <;> simp [CPS.Ren.toSub, subst, ren, ← CPS.Ren.toSub_lift, *]
-  -- case var h => cases h; rfl
-
-def CPS.Sub.comp (σ₁ : Sub Γ Δ) (σ₂ : Sub Δ Φ) : Sub Γ Φ :=
-  fun n => (σ₂ n).subst σ₁
-
-@[simp]
-theorem CPS.Sub.wk_snoc_zero (σ : Sub Γ Δ) : (σ.wk (A := A)).snoc Expr.zero = σ.lift := rfl
-
-@[simp]
-theorem CPS.Expr.subst_lift_zero (σ : Sub Γ Δ) : σ.lift (A := A) ⟨0,h⟩ = Expr.zero := rfl
-
-@[simp]
-theorem CPS.Expr.subst_snoc_zero (σ : Sub Γ Δ) : σ.snoc e ⟨0,h⟩ = e := rfl
-
-@[simp]
-theorem CPS.Expr.subst_snoc_succ (σ : Sub Γ Δ) : σ.snoc e ⟨n+1,h⟩ = σ ⟨n,Nat.lt_of_succ_lt_succ h⟩ := rfl
-
-@[simp]
-theorem CPS.Expr.subst_lift_succ (σ : Sub Γ Δ) : σ.lift (A := A) ⟨n+1,h⟩ = (σ ⟨n,Nat.lt_of_succ_lt_succ h⟩).lift := rfl
-
-theorem CPS.Sub.ren_comp_lift {r : Ren Γ Δ} {σ : Sub Δ Φ} : (σ.ren_comp r).lift (A := A) = σ.lift.ren_comp r.lift  := by
-  funext ⟨x,_⟩
-  simp
-  cases x
-  · rfl
-  · simp [ren_comp, Expr.lift, Expr.ren_of_ren_ren]
-    rfl
-
-theorem CPS.Sub.wk_of_lift_comp_ren_wk {σ : Sub Γ Δ} : (σ.lift.comp_ren Ren.wk) = σ.wk (A := A) := by
-  funext ⟨x,_⟩
-  rw [comp_ren, Sub.wk, Expr.lift, Ren.wk]
-  simp only
-  unfold Fin.succ
-  rw [CPS.Expr.subst_lift_succ, Expr.lift]
-
-theorem CPS.Sub.head (σ : Sub Γ Δ) : Expr.subst (σ.snoc t) Expr.zero = t := rfl
-theorem CPS.Sub.tail (σ : Sub Γ Δ) : (σ.snoc t).comp Sub.id.wk = σ := rfl
-
-theorem CPS.Sub.eta (σ : Sub Γ (A::Δ)) : (σ.comp Sub.id.wk).snoc (σ 0) = σ := by
-  funext ⟨n,_⟩
-  cases n <;> rfl
-
-theorem CPS.Sub.Zshift' : Sub.id.wk.snoc Expr.zero = @Sub.id (A::Γ) := by
-  funext ⟨n,_⟩
-  cases n <;> rfl
-
-theorem CPS.Sub.Zshift : Sub.id.lift = @Sub.id (A::Γ) := Zshift'
-
-theorem CPS.Sub.idR (σ : Sub Γ Δ) : (σ.comp Sub.id) = σ := rfl
-
-@[simp]
-theorem CPS.Expr.subst_id : Expr.subst Sub.id t = t := by
-  induction t <;> simp [CPS.Sub.Zshift, subst, *]
-  case var h => cases h; rfl
-
-@[simp]
-theorem CPS.Sub.idL (σ : Sub Γ Δ) : Sub.comp Sub.id σ = σ := by
-  funext n
-  apply CPS.Expr.subst_id
-
--- ext-sub-ren-∘≣
-theorem CPS.Expr.subst_comp_ren_lift (σ : Sub Δ Γ ) (ρ : Ren Φ Δ) : (σ.ren_comp ρ).lift (A := A) = (σ.lift.ren_comp ρ.lift ) := by
-  funext ⟨n,_⟩
-  cases n
-  · rfl
-  · simp [Sub.ren_comp, Expr.lift, ren_of_ren_ren]
-    rfl
-
--- sub-ren-∘-≡
-theorem CPS.Expr.subst_ren (t : Expr Φ t A) (ρ : Ren Γ Δ) (σ : Sub Δ Φ) : (t.subst σ).ren ρ = t.subst (σ.ren_comp ρ) := by
-  induction t generalizing ρ Γ Δ <;> simp [Sub.ren_comp, ren, subst, *]
-  case var h => cases h; rfl
-  case lam ih =>
-    have := ih ρ.lift σ.lift
-    rw [← this, CPS.Expr.subst_comp_ren_lift]
-    assumption
-  case and_elim ih₁ ih₂ =>
-    rw [CPS.Expr.subst_comp_ren_lift, CPS.Expr.subst_comp_ren_lift]
-
-@[simp]
-theorem CPS.Ren.lift_succ (ρ : Ren Γ Δ) : (ρ.lift (A := A)).val ⟨n+1,h⟩ = (ρ.val ⟨n, Nat.lt_of_succ_lt_succ h⟩).succ := rfl
-
-@[simp]
-theorem CPS.Sub.lift_succ (σ : Sub Γ Δ) : (σ.lift (A := A)) n.succ = (σ n).lift := rfl
-
---  ext-ren-sub-∘≣, just cases n <;> rfl in agda *somehow*
-theorem CPS.Expr.ren_comp_subst_lift (ρ : Ren Δ Γ) (σ : Sub Φ Δ) : (σ.comp_ren ρ).lift (A := A) = (σ.lift.comp_ren ρ.lift) := by
-  funext ⟨n,_⟩
-  cases n
-  case zero => rfl
-  case succ n h =>
-    simp [Sub.comp_ren, Expr.lift]
-    grind
-
-theorem CPS.Expr.ren_subst (t : Expr Φ t A) (σ : Sub Γ Δ) (ρ : Ren  Δ Φ) : (t.ren ρ).subst σ = t.subst (Sub.comp_ren σ ρ) := by
-  induction t generalizing σ Γ Δ <;> simp [Sub.comp_ren, ren, subst, *]
-  case var h => cases h; rfl
-  case lam ih =>
-    have := ih σ.lift ρ.lift
-    rw [← this, ren_comp_subst_lift]
-    assumption
-  case and_elim ih₁ ih₂ =>
-    rw [ren_comp_subst_lift, ren_comp_subst_lift]
-
-theorem CPS.Expr.lift_subst_lift (t : Expr Δ t B) (σ : Sub Γ Δ) :
-(t.lift (A := B)).subst σ.lift = (t.subst σ).lift (B := A) := by
-  induction t <;> simp [Expr.lift, Expr.ren, Expr.subst] at *
-  case var h => cases h; rfl
-  case lam ih =>
-    rw [Expr.subst_ren, ← Expr.subst_comp_ren_lift, Expr.ren_subst, ← Expr.ren_comp_subst_lift]
-    rfl
-  case and_elim ih₁ ih₂ =>
-    constructor
-    · rw [Expr.subst_ren, Expr.ren_subst]
-      rfl
-    · rw [Expr.subst_ren, ← Expr.subst_comp_ren_lift, Expr.ren_subst, ← Expr.ren_comp_subst_lift, ← Expr.ren_comp_subst_lift , ← Expr.subst_comp_ren_lift]
-      congr 1
-  case app ih₁ ih₂ | and_intro ih₁ ih₂ => exact ⟨ih₁ _, ih₂ _⟩
-
-@[simp]
-theorem CPS.Sub.comp_lift {σ : Sub Γ Δ} {τ : Sub Δ Φ} : Sub.comp σ.lift τ.lift = (Sub.comp σ τ).lift (A := A) := by
-  funext ⟨x,_⟩
-  cases x --generalizing  Γ Δ Φ
-  case zero => rfl
-  case succ n h =>
-    simp [Sub.comp, Expr.lift, CPS.Expr.ren_subst , CPS.Expr.subst_ren]
-    rfl
-
-theorem CPS.Expr.subst_subst  {σ₁ : Sub Γ Δ} {σ₂ : Sub Δ Φ} (v : Expr Φ t A) : (v.subst σ₂).subst σ₁ = v.subst (σ₁.comp σ₂) := by
-  induction v generalizing σ₁ Γ Δ <;> simp only [subst, Fin.getElem_fin, Sub.comp, *]
-  case var h =>
-    cases h
-    rfl
-  case lam A Φ t ih =>
-    rw [Sub.comp_lift]
-  case and_elim ih =>
-    rw [Sub.comp_lift, Sub.comp_lift]
-
-theorem CPS.Expr.cast_val {h : Γ[n] = A}(e : A = B) : e ▸ Expr.var n h = Expr.var n h' := by cases e; rfl
-
-theorem CPS.Equiv.ren {r : Ren Γ Δ} (e₁ e₂ : Expr Δ t A) : Equiv e₁ e₂ → Equiv (e₁.ren r) (e₂.ren r) := by
-  intro h
-  induction h generalizing Γ
-  case refl => exact .refl
-  case symm ih => exact .symm ih
-  case trans ih₁ ih₂ => exact .trans ih₁ ih₂
-  case lam ih => exact Equiv.lam ih
-  case app ih₁ ih₂ => exact Equiv.app ih₁ ih₂
-  case and_intro ih₁ ih₂ => exact Equiv.and_intro ih₁ ih₂
-  case and_elim ih₁ ih₂ => exact Equiv.and_elim ih₁ ih₂
-  case eta v =>
-    simp [Expr.ren, Expr.zero, Expr.lift_ren_lift]
-    exact Equiv.eta (v := (Expr.ren r v))
-  case eta_and Δ t fst snd e =>
-    simp [Expr.ren]
-    apply Equiv.trans
-    · apply Equiv.eta_and
-    · have : (e.ren r.lift.lift).subst ((Sub.id.snoc (Expr.ren r snd)).snoc (Expr.ren r fst)) = (e.subst ((Sub.id.snoc snd).snoc fst)).ren r := by
-        simp [Expr.subst_ren, Expr.ren_subst]
-        congr 1
-        funext ⟨x,_⟩
-        cases x
-        case zero => rfl
-        case succ x h =>
-          cases x
-          · rfl
-          · cbv
-            apply Expr.cast_val
-      rw [this]
-      apply Equiv.refl
-  case beta =>
-    simp [Expr.ren]
-    apply Equiv.trans
-    · apply Equiv.beta
-    · rename_i e v
-      have : (e.ren r.lift).subst (Sub.id.snoc (Expr.ren r v)) = (e.subst (Sub.id.snoc v)).ren r := by
-        simp [Expr.subst_ren, Expr.ren_subst]
-        congr 1
-        funext ⟨x,_⟩
-        cases x
-        case zero => rfl
-        case succ x h =>
-          cbv
-          apply Expr.cast_val
-      rw [this]
-      apply Equiv.refl
-
-theorem CPS.Equiv.subst {σ : Sub Γ Δ} (e₁ e₂ : CPS.Expr Δ t A)  : CPS.Equiv e₁ e₂ → CPS.Equiv (e₁.subst σ) (e₂.subst σ) := by
-  intro h
-  induction h generalizing Γ
-  case refl => exact .refl
-  case symm ih => exact .symm ih
-  case trans ih₁ ih₂ => exact .trans ih₁ ih₂
-  case lam ih => exact CPS.Equiv.lam ih
-  case app ih₁ ih₂ => exact CPS.Equiv.app ih₁ ih₂
-  case and_intro ih₁ ih₂ => exact CPS.Equiv.and_intro ih₁ ih₂
-  case and_elim ih₁ ih₂ => exact CPS.Equiv.and_elim ih₁ ih₂
-  case eta v =>
-    simp [Expr.subst, Expr.zero, CPS.Expr.lift_subst_lift]
-    exact CPS.Equiv.eta (v := (Expr.subst σ v))
-  case eta_and =>
-    simp [Expr.subst]
-    apply CPS.Equiv.trans
-    · apply CPS.Equiv.eta_and
-    · rename_i fst snd e
-      have : (Expr.subst ((Sub.id.snoc (Expr.subst σ snd)).snoc (Expr.subst σ fst)) (Expr.subst σ.lift.lift e)) = (Expr.subst σ (Expr.subst ((Sub.id.snoc snd).snoc fst) e)) := by
-        simp [Expr.subst_subst]
-        congr 1
-        funext ⟨n,_⟩
-        cases n
-        case zero => rfl
-        case succ n _ =>
-          simp [Sub.comp, Sub.lift]
-          cases n
-          · rfl
-          · simp [Sub.id, Expr.subst, Expr.lift, Expr.ren_subst]
-      rw [this]
-      apply CPS.Equiv.refl
-  case beta =>
-    simp [Expr.subst]
-    apply CPS.Equiv.trans
-    · apply CPS.Equiv.beta
-    · rename_i e v
-      have : (Expr.subst (Sub.id.snoc (Expr.subst σ v)) (Expr.subst σ.lift e)) = (Expr.subst σ (Expr.subst (Sub.id.snoc v) e)) := by
-        simp [Expr.subst_subst]
-        congr 1
-        funext ⟨n,_⟩
-        cases n
-        · rfl
-        · simp [Sub.comp, Sub.lift, Sub.id, Expr.subst, Expr.lift, Expr.ren_subst]
-      rw [this]
-      apply CPS.Equiv.refl
-
-theorem CPS.Equiv.cast  (h₁ : Expr Γ t A = Expr Γ t B) (h₂ : A = B) (e₁ e₂ : CPS.Expr Γ t A) : CPS.Equiv e₁ e₂ →
-  CPS.Equiv (cast h₁ e₁) (cast h₁ e₂) := by
-  cases h₂
-  cases h₁
-  exact id
+-- def STLC.Expst.subst_toCPS (σ : Sub Γ Δ) : (Expr.subst σ t).toCPS = CPS.Expr.subst σ.toCPS t.toCPS
 
 theorem STLC.Equiv.toCPS (e e' : Expr Γ t A) (h : Equiv e e') : CPS.Equiv e.toCPS e'.toCPS := by
   induction h
